isabelle/AbstractBindingTrees.thy
@@ -29,13 +29,13 @@ fun subst_zero :: "'op ABT \<Rightarrow> var \<Rightarrow> 'op ABT" where
 abbreviation subst_one :: "'op ABT \<Rightarrow> 'op ABT \<Rightarrow> 'op ABT" ("_[_]" 70) where
   "subst_one N M \<equiv> \<llangle> subst_zero M \<rrangle> N"
 
-definition seqss :: "('op ABT) sub \<Rightarrow> ('op ABT) sub \<Rightarrow> ('op ABT) sub" (infixl ";" 60) where
+definition seqss :: "('op ABT) sub \<Rightarrow> ('op ABT) sub \<Rightarrow> ('op ABT) sub" (infixr ";" 70) where
   "(\<sigma> ; \<tau>) x \<equiv> \<llangle>\<tau>\<rrangle> (\<sigma> x)"
 
-definition seqrs :: "var sub \<Rightarrow> ('op ABT) sub \<Rightarrow> ('op ABT) sub" ("_ r; _") where
+definition seqrs :: "var sub \<Rightarrow> ('op ABT) sub \<Rightarrow> ('op ABT) sub" (infixr "r;" 70) where
   "(\<rho> r; \<tau>) x \<equiv> \<tau> (\<rho> x)"
 
-definition seqsr :: "('op ABT) sub \<Rightarrow> var sub \<Rightarrow> ('op ABT) sub" ("_ ;r _") where
+definition seqsr :: "('op ABT) sub \<Rightarrow> var sub \<Rightarrow> ('op ABT) sub" (infixr ";r" 70) where
   "(\<sigma> ;r \<rho>) x \<equiv> rename \<rho> (\<sigma> x)"
 
 definition id :: "('op ABT) sub" where
@@ -77,10 +77,24 @@ theorem subst_id[simp]: "\<llangle>id\<rrangle> M = M"
 theorem IdR[simp]: "\<sigma> ; id = \<sigma>"
   unfolding seqss_def by (rule ext) simp
 
-theorem ConsSeq[simp]: "(M \<bullet> \<sigma>); \<tau> = \<llangle> \<tau> \<rrangle> M \<bullet> (\<sigma> ; \<tau>)"
+theorem ConsSeq[simp]: "(M \<bullet> \<sigma>) ; \<tau> = \<llangle> \<tau> \<rrangle> M \<bullet> (\<sigma> ; \<tau>)"
   apply (rule ext)
   apply (case_tac x)
   unfolding seqss_def apply simp 
+  apply simp
+  done
+
+theorem ConsSeqRS[simp]: "(y \<bullet> \<rho>) r; \<tau> = \<tau> y \<bullet> (\<rho> r; \<tau>)"
+  apply (rule ext)
+  apply (case_tac x)
+  unfolding seqrs_def apply simp
+  apply simp
+  done
+
+theorem ConsSeqSR[simp]: "(M \<bullet> \<sigma>) ;r \<rho> = rename \<rho> M \<bullet> (\<sigma> ;r \<rho>)"
+  apply (rule ext)
+  apply (case_tac x)
+  unfolding seqsr_def apply simp
   apply simp
   done
 
@@ -119,20 +133,37 @@ lemma lift_seq_up: "abt_s.lift_sub \<sigma> = \<sigma> ; \<up>"
   apply (rule ext)
   unfolding seqss_def shift_def using rename_subst[of Suc] apply auto done
 
-lemma ren_suc_shift[simp]: "\<lceil>Suc\<rceil> = \<up>"
+lemma ren_suc_shift: "\<lceil>Suc\<rceil> = \<up>"
   unfolding shift_def by simp
+
+lemma exts_cons_seq: "exts \<sigma> = Var 0 \<bullet> (\<sigma> ; \<up>)"
+proof -
+  have 1: "(\<lambda> x. rename Suc (\<sigma> x)) = (\<lambda> x. \<llangle> \<lceil> Suc \<rceil> \<rrangle> (\<sigma> x))"
+    using rename_subst[of Suc] by auto
+  have "exts \<sigma> = Var 0 \<bullet> (\<lambda> x. \<llangle> \<lceil> Suc \<rceil> \<rrangle> (\<sigma> x))" using 1 by simp
+  also have "... = Var 0 \<bullet> (\<sigma> ; \<up>)" unfolding seqss_def by simp
+  finally show "exts \<sigma> = Var 0 \<bullet> (\<sigma> ; \<up>)" .
+qed
 
 interpretation rss:
   substable3 "Var 0" Suc "\<lambda>x. x" Var "rename Suc" "\<lambda>x. x" Var "rename Suc" "\<lambda>x. x" Var
   by unfold_locales 
 
-lemma rss_comp_cong_ext: "\<rho> r; \<sigma> = \<tau> \<Longrightarrow>
-       rss.comp_cong (abt_s.ext \<sigma>) (extr \<rho>) (abt_s.ext \<tau>)"
-  unfolding extr_def apply clarify
-  apply (case_tac x)
-  apply simp 
-   apply (simp add: seqrs_def)
-  done
+theorem ShiftConsRS[simp]: "Suc r; (M \<bullet> \<sigma>) = \<sigma>"
+  unfolding cons_def subst_def seqrs_def shift_def by simp
+
+theorem assoc_RRS[simp]: "(\<rho> r;r \<sigma>) r; \<tau> = \<rho> r; (\<sigma> r; \<tau>)"
+  unfolding seqrr_def seqrs_def by auto
+
+theorem assoc_RSS[simp]: "(\<rho> r; \<sigma>) ; \<tau> = \<rho> r; (\<sigma> ; \<tau>)"
+  unfolding seqrs_def seqss_def by auto
+
+lemma rss_comp_cong_ext: assumes 1: "\<rho> r; \<sigma> = \<tau>" shows "(extr \<rho>) r; (exts \<sigma>) = (exts \<tau>)"
+proof (simp add: exts_cons_seq)
+  have "Var 0 \<bullet> (\<rho> r; \<sigma> ; \<lceil>Suc\<rceil>) = Var 0 \<bullet> ((\<rho> r; \<sigma>) ; \<lceil>Suc\<rceil>)" by simp
+  also have "... = Var 0 \<bullet> (\<tau> ; \<lceil>Suc\<rceil>)" using 1 by simp
+  finally show "Var 0 \<bullet> (\<rho> r; \<sigma> ; \<lceil>Suc\<rceil>) = Var 0 \<bullet> (\<tau> ; \<lceil>Suc\<rceil>)" .
+qed
 
 lemma rsscc_eq_seqrs: "(\<rho> r; \<sigma> = \<tau>) = (rss.comp_cong \<sigma> \<rho> \<tau>)" 
   unfolding seqrs_def by auto
@@ -141,73 +172,104 @@ theorem subst_rename_fusion:
   assumes 1: "\<rho> r; \<sigma> = \<tau>"
   shows "\<llangle>\<sigma>\<rrangle> (rename \<rho> M) = \<llangle>\<tau>\<rrangle> M"
 proof -
-  have 2: "rss.comp_cong \<sigma> \<rho> \<tau>" using 1 unfolding seqrs_def by auto
+  have 2: "rss.comp_cong \<sigma> \<rho> \<tau>" using 1 rsscc_eq_seqrs by fast
   {
     fix \<sigma>::"var sub" and \<tau> :: "('op ABT) sub" and \<rho> x
     assume 4: "rss.comp_cong \<tau> \<sigma> \<rho>"
-    then have "\<sigma> r; \<tau> = \<rho>" unfolding seqrs_def by simp
-    then have "rss.comp_cong (abt_s.ext \<tau>) (extr \<sigma>) (abt_s.ext \<rho>)"
+    then have "\<sigma> r; \<tau> = \<rho>" using rsscc_eq_seqrs by fast
+    then have 1: "(extr \<sigma>) r; (exts \<tau>) = (exts \<rho>)"
       by (rule rss_comp_cong_ext) 
+    have "rss.comp_cong (abt_s.ext \<tau>) (var_s.ext \<sigma>) (abt_s.ext \<rho>)"
+      apply auto apply (case_tac x) apply force apply (auto simp add: exts_cons_seq)
+    proof -
+      fix x
+      have "((extr \<sigma>) r; (exts \<tau>)) (Suc x) = (exts \<rho>) (Suc x)" using 1 by simp
+      then have "(\<sigma> r; \<tau> ; \<lceil>Suc\<rceil>) x = (\<rho> ; \<lceil>Suc\<rceil>) x" by (simp add: exts_cons_seq)
+      then show "(\<tau> ; \<lceil>Suc\<rceil>) (\<sigma> x) = (\<rho> ; \<lceil>Suc\<rceil>) x" unfolding seqrs_def by simp
+    qed      
   }
   then have 3: "\<forall>\<sigma> \<tau> \<rho>. rss.comp_cong \<tau> \<sigma> \<rho> \<longrightarrow> rss.comp_cong (exts \<tau>) (var_s.ext \<sigma>) (exts \<rho>)"
-    unfolding extr_def by blast
-  have "abt_s.map_abt \<sigma> (var_s.map_abt \<rho> M) = abt_s.map_abt \<tau> M"
-    apply (rule rss.map_fusion)
-    using 2 apply fast
-    using 3 apply blast
-    done
-  then show ?thesis unfolding subst_def rename_def apply simp done  
+     by blast
+  from 2 3 have "abt_s.map_abt \<sigma> (var_s.map_abt \<rho> M) = abt_s.map_abt \<tau> M"
+    by (rule rss.map_fusion)
+  then show ?thesis unfolding subst_def rename_def by simp  
 qed
 
-
-(*
-
-
-
-
+theorem assoc_SRS[simp]: "(\<sigma> ;r \<rho>) ; \<tau> = \<sigma> ; (\<rho> r; \<tau>)"
+  unfolding seqsr_def seqss_def seqrs_def apply (rule ext)
+  apply (rule subst_rename_fusion)
+  unfolding seqrs_def apply simp
+  done
 
 
 interpretation srs: 
   substable3 "Var 0" 
-  "rename Suc" Var "\<lambda> x. x" 
-  Suc Var "\<lambda> x. x"
-  "rename Suc" "\<lambda> x. x" Var
+    "rename Suc" Var "\<lambda> x. x" 
+    Suc Var "\<lambda> x. x"
+    "rename Suc" "\<lambda> x. x" Var
   by unfold_locales
 
-lemma srscc_eq_seqsr[simp]: "(\<sigma> ;r \<rho> = \<tau>) = (srs.comp_cong \<rho> \<sigma> \<tau>)" by auto
+lemma srscc_eq_seqsr: "(\<sigma> ;r \<rho> = \<tau>) = (srs.comp_cong \<rho> \<sigma> \<tau>)" 
+  unfolding seqsr_def rename_def by auto
 
 lemma srs_comp_cong_ext: fixes x :: var
   assumes cc: "\<sigma> ;r \<rho> = \<tau>"
   shows "rename (extr \<rho>) (exts \<sigma> x) = exts \<tau> x"
 proof (cases x)
   case 0
-  then show ?thesis by (simp add: cons_def)
+  then show ?thesis by simp 
 next
   case (Suc y)
   have            "((exts \<sigma>) ;r (extr \<rho>)) x 
-                 = rename (extr \<rho>) (rename Suc (\<sigma> y))" using Suc by (simp add: cons_def)
-  also have "... = rename (Suc r;r (extr \<rho>)) (\<sigma> y)" using rename_fusion[of "(extr \<rho>)" Suc "(\<lambda> x. (extr \<rho>) (Suc x))" "\<sigma> y"] by fast
-  also have "... = rename (\<rho> r;r Suc) (\<sigma> y)" by (simp add: cons_def)
-  also have "... = rename Suc (rename \<rho> (\<sigma> y))" using rename_fusion[of Suc \<rho> "\<rho> r;r Suc" "\<sigma> y"] by auto
-  also have "... = rename Suc (\<tau> y)" using cc by auto
+                 = rename (extr \<rho>) (rename Suc (\<sigma> y))" using Suc seqsr_def by auto
+  also have "... = rename (Suc r;r (extr \<rho>)) (\<sigma> y)" 
+    by (rule rename_fusion[of "(extr \<rho>)" Suc "\<sigma> y"])
+  also have "... = rename (\<rho> r;r Suc) (\<sigma> y)" by simp
+  also have "... = rename Suc (rename \<rho> (\<sigma> y))" using rename_fusion[of Suc \<rho> "\<sigma> y"] by auto
+  also have "... = rename Suc ((\<sigma> ;r \<rho>) y)" unfolding seqsr_def ..
+  also have "... = rename Suc (\<tau> y)" using cc by simp
   also have "... = exts \<tau> x" using Suc by (simp add: cons_def)
-  finally show ?thesis .
+  finally have "((exts \<sigma>) ;r (extr \<rho>)) x = exts \<tau> x" by simp
+  then show ?thesis unfolding seqsr_def by simp
 qed
 
 (* This could instead be rename_map_fusion (more generic) *)
-theorem rename_subst_fusion:
-  assumes 1: "srs.comp_cong \<rho> \<sigma> \<tau>"
-  shows "rename \<rho> (\<llangle>\<sigma>\<rrangle> M) = \<llangle>\<tau>\<rrangle> M"
-  unfolding subst_def apply (rule srs.map_fusion)
-  using 1 apply fast
-  using srs_comp_cong_ext apply auto
-  done
+
+theorem rename_subst_fusion: "rename \<rho> (\<llangle>\<sigma>\<rrangle> M) = \<llangle>\<sigma> ;r \<rho>\<rrangle> M"
+proof -
+  have rst: "\<sigma> ;r \<rho> = \<sigma> ;r \<rho>" by simp
+  have "srs.comp_cong \<rho> \<sigma> (\<sigma> ;r \<rho>)" unfolding seqsr_def rename_def by simp 
+  then have "var_s.map_abt \<rho> (abt_s.map_abt \<sigma> M) = abt_s.map_abt (\<sigma> ;r \<rho>) M"
+  proof (rule srs.map_fusion, clarify)
+    fix \<sigma> \<tau> \<rho> x assume "srs.comp_cong \<tau> \<sigma> \<rho>"
+    then have "\<sigma> ;r \<tau> = \<rho>" unfolding seqsr_def rename_def by auto
+    then have "rename (extr \<tau>) (exts \<sigma> x) = exts \<rho> x" by (rule srs_comp_cong_ext)
+    then show "var_s.map_abt (var_s.ext \<tau>) (exts \<sigma> x) = exts \<rho> x"
+      unfolding rename_def extr_def by fast
+  qed
+  then show "rename \<rho> (\<llangle>\<sigma>\<rrangle> M) = \<llangle>\<sigma> ;r \<rho>\<rrangle> M"
+    unfolding rename_def subst_def by fast
+qed
+
+theorem assoc_SSR[simp]: "(\<sigma> ; \<tau>) ;r \<rho> = \<sigma> ; (\<tau> ;r \<rho>)"
+proof (rule ext)
+  fix x
+  have "((\<sigma> ; \<tau>) ;r \<rho>) x = rename \<rho> (\<llangle>\<tau>\<rrangle> (\<sigma> x))" 
+    unfolding seqsr_def seqss_def by simp
+  also have "... = \<llangle>\<tau> ;r \<rho>\<rrangle> (\<sigma> x)"
+    by (rule rename_subst_fusion)
+  also have "... = (\<sigma> ; (\<tau> ;r \<rho>)) x"
+    unfolding seqss_def ..
+  finally show "((\<sigma> ; \<tau>) ;r \<rho>) x = (\<sigma> ; (\<tau> ;r \<rho>)) x" .
+qed
 
 interpretation sss: 
   substable3 "Var 0" "rename Suc" Var "\<lambda> x. x"
    "rename Suc" "\<lambda> x. x" Var
    "rename Suc" "\<lambda> x. x" Var
   by unfold_locales
+
+(*
 
 lemma ssscc_eq_seqss: "(\<sigma> ; \<rho> = \<tau>) = (sss.comp_cong \<rho> \<sigma> \<tau>)"
   unfolding subst_def by auto
